formal/Value.thy
@@ -27,15 +27,15 @@ lemma MaybeBoolInt_not_num_1: "\<forall>n. r \<noteq> Some (Num n) \<Longrightar
   apply (case_tac a)
   by auto
 
-definition ValueGt :: "value option \<Rightarrow> value option \<Rightarrow> trilean"  where
-  "ValueGt a b \<equiv> MaybeBoolInt (\<lambda>x::int.\<lambda>y::int.(x>y)) a b"
+definition value_gt :: "value option \<Rightarrow> value option \<Rightarrow> trilean"  where
+  "value_gt a b \<equiv> MaybeBoolInt (\<lambda>x::int.\<lambda>y::int.(x>y)) a b"
 
-definition ValueLt :: "value option \<Rightarrow> value option \<Rightarrow> trilean"  where
-  "ValueLt a b \<equiv> MaybeBoolInt (\<lambda>x::int.\<lambda>y::int.(x<y)) a b"
+definition value_lt :: "value option \<Rightarrow> value option \<Rightarrow> trilean"  where
+  "value_lt a b \<equiv> MaybeBoolInt (\<lambda>x::int.\<lambda>y::int.(x<y)) a b"
 
-definition ValueEq :: "value option \<Rightarrow> value option \<Rightarrow> trilean"  where
-  "ValueEq a b \<equiv> (if a = b then true else false)"
-declare ValueEq_def [simp]
+definition value_eq :: "value option \<Rightarrow> value option \<Rightarrow> trilean"  where
+  "value_eq a b \<equiv> (if a = b then true else false)"
+declare value_eq_def [simp]
 
 instantiation "value" :: linorder begin
 fun less_eq_value :: "value \<Rightarrow> value \<Rightarrow> bool" where
